theories/lang_oadt/metatheories.v
@@ -44,4 +44,25 @@ Proof.
 Qed.
 
 (** ** Obliviousness *)
-(* TODO: the obliviousness corollary for trace. *)
+
+(* Essentially a noninterference theorem. Indistinguishable well-typed
+expressions can always take the same steps and new expressions remain
+indistinguishable. *)
+Theorem obliviousness Σ e1 e1' e2 τ τ' n :
+  Σ; e1 ▷ τ ->
+  Σ; e1' ▷ τ' ->
+  Σ ⊨ e1 -->{n} e2 ->
+  e1 ≈ e1' ->
+  (exists e2', Σ ⊨ e1' -->{n} e2') /\
+  (forall e2', Σ ⊨ e1' -->{n} e2' -> e2 ≈ e2').
+Proof.
+  intros [Hd Ht1] [_ Ht1']. apply gdefs_typing_wf in Hd.
+  intros H. revert dependent e1'.
+  induction H; intros.
+  - hauto ctrs: trans_ext inv: trans_ext.
+  - edestruct obliviousness_step as [[??] ?]; eauto.
+    split; intros.
+    + hauto ctrs: trans_ext use: preservation.
+    + select (_ ⊨ _ -->{_} _) (fun H => sinvert H).
+      qauto use: preservation.
+Qed.
